Faster denote

tests/lean/run/rsimp_linear.lean
@@ -3,6 +3,109 @@ import Std.Tactic.RSimp.ConvTheorem
 
 import Lean
 
+namespace Data
+
+/-!
+A data structure for modelling `Fin n → α` (or `Array α`) optimized for a fast kernel-reduction get
+operation.
+
+For now not universe-polymorphic; smaller proof objects and no complication with the `ToExpr` type
+class.
+-/
+
+inductive RArray (α : Type) : Type  where
+  | leaf : α → RArray α
+  | branch : Nat → RArray α → RArray α → RArray α
+
+variable {α : Type}
+
+/-- The crucial operation, written with very little abstractional overhead -/
+noncomputable def RArray.get (a : RArray α) (n : Nat) : α :=
+  RArray.rec (fun x => x) (fun p _ _ l r => (Nat.ble p n).rec l r) a
+
+theorem RArray.get_eq_def (a : RArray α) (n : Nat) :
+  a.get n = match a with
+    | .leaf x => x
+    | .branch p l r => (Nat.ble p n).rec (l.get n) (r.get n) := by
+  conv => lhs; unfold RArray.get
+  split <;> rfl
+
+def RArray.getImpl (a : RArray α) (n : Nat) : α :=
+  match a with
+  | .leaf x => x
+  | .branch p l r => if n < p then l.getImpl n else r.getImpl n
+
+@[csimp]
+theorem RArray.get_eq_getImpl : @RArray.get = @RArray.getImpl := by
+  ext α a n
+  induction a with
+  | leaf _ => rfl
+  | branch p l r ihl ihr =>
+    rw [RArray.getImpl, RArray.get_eq_def]
+    simp only [ihl, ihr]
+    cases hnp : Nat.ble p n
+    · replace hnp := ne_true_of_eq_false hnp
+      simp at hnp
+      rw [if_pos]
+      omega
+    · simp at hnp
+      rw [if_neg]
+      omega
+
+instance : GetElem (RArray α) Nat α (fun _ _ => True) where
+  getElem a n _ := a.get n
+
+def RArray.size : RArray α → Nat
+  | leaf _ => 1
+  | branch _ l r => l.size + r.size
+
+def RArray.ofFn {n : Nat} (f : Fin n → α) (h : 0 < n) : RArray α :=
+  go 0 n h (Nat.le_refl _)
+where
+  go (lb ub : Nat) (h1 : lb < ub) (h2 : ub ≤ n) : RArray α :=
+    if h : lb + 1 = ub then
+      .leaf (f ⟨lb, Nat.lt_of_lt_of_le h1 h2⟩)
+    else
+      let mid := (lb + ub)/2
+      .branch mid (go lb mid (by omega) (by omega)) (go mid ub (by omega) h2)
+
+def RArray.ofArray (xs : Array α) (h : 0 < xs.size) : RArray α :=
+  .ofFn (fun i => xs.get i) h
+
+theorem RArray.ofFn_correct {n : Nat} (f : Fin n → α) (h : 0 < n) (i : Fin n):
+    RArray.get (.ofFn f h) i = f i :=
+  go 0 n h (Nat.le_refl _) (Nat.zero_le _) i.2
+where
+  go lb ub h1 h2 (h3 : lb ≤ i.val) (h3 : i.val < ub) : RArray.get (.ofFn.go f lb ub h1 h2) i = f i := by
+    induction lb, ub, h1, h2 using RArray.ofFn.go.induct (f := f) (n := n)
+    case case1 =>
+      simp [ofFn.go, RArray.get_eq_getImpl, RArray.getImpl]
+      congr
+      omega
+    case case2 ih1 ih2 hiu =>
+      rw [ofFn.go]; simp only [↓reduceDIte, *]
+      simp [RArray.get_eq_getImpl, RArray.getImpl] at *
+      split
+      · rw [ih1] <;> omega
+      · rw [ih2] <;> omega
+
+
+section Meta
+open Lean
+
+def RArray.toExpr (ty : Expr) (f : α → Expr) : RArray α → Expr
+  | .leaf x       =>
+    mkApp2 (mkConst ``RArray.leaf) ty (f x)
+  | .branch p l r =>
+    mkApp4 (mkConst ``RArray.branch) ty (.lit (.natVal p)) (l.toExpr ty f) (r.toExpr ty f)
+
+instance [ToExpr α] : ToExpr (RArray α) where
+  toExpr a := a.toExpr (toTypeExpr α) (toExpr ·)
+  toTypeExpr := mkApp (mkConst ``RArray) (toTypeExpr α)
+
+end Meta
+end Data
+
 open Nat.Linear
 
 section sortFuse
@@ -126,6 +229,17 @@ theorem Nat.Linear.Expr.toPoly_eq_toPolyFast :
 
 end ToPoly
 
+section AltDenote
+
+def Nat.Linear.Expr.denote' (ctx : Data.RArray Nat) : Expr → Nat
+  | Expr.add a b  => Nat.add (denote' ctx a) (denote' ctx b)
+  | Expr.num k    => k
+  | Expr.var v    => ctx.get v
+  | Expr.mulL k e => Nat.mul k (denote' ctx e)
+  | Expr.mulR e k => Nat.mul (denote' ctx e) k
+
+end AltDenote
+
 -- theorem Nat.beq_eq' (a b : Nat) : (a == b) = Nat.beq a b := sorry
 
 attribute [rsimp ←] Nat.beq_eq Nat.mul_eq Nat.add_eq Bool.cond_decide
@@ -142,14 +256,14 @@ attribute [rsimp_optimize] Nat.Linear.Poly.insertSorted
 attribute [rsimp_optimize] Nat.Linear.Poly.sort.go
 attribute [rsimp_optimize] Nat.Linear.Poly.sort
 attribute [rsimp_optimize] Nat.Linear.Poly.fuse
+attribute [rsimp_optimize] Nat.Linear.Expr.toPolyAux
+attribute [rsimp_optimize] Nat.Linear.Expr.toPolyFast
 
 -- This is actually a bit slower, it seems
 -- But faster if there are repeated variables
 attribute [rsimp] Nat.Linear.Poly.norm_eq_sortFuse
 -- attribute [rsimp_optimize] Nat.Linear.Poly.norm
 
-attribute [rsimp_optimize] Nat.Linear.Expr.toPolyAux
-attribute [rsimp_optimize] Nat.Linear.Expr.toPolyFast
 
 -- attribute [rsimp_optimize] Nat.Linear.Expr.toPoly
 attribute [rsimp] Nat.Linear.Expr.toPoly_eq_toPolyFast
@@ -161,6 +275,7 @@ attribute [rsimp_optimize] Nat.Linear.Poly.cancel
 
 attribute [rsimp_optimize] Nat.Linear.Var.denote.go
 attribute [rsimp_optimize] Nat.Linear.Var.denote
+-- set_option trace.tactic.rsimp_optimize true in
 attribute [rsimp_optimize] Nat.Linear.Expr.denote
 
 /-- A hook to use below, and to easily swap out the definition -/
@@ -197,62 +312,100 @@ theorem Nat.Linear.Expr.of_cancel_eq_opt_denote (ctx : Context) (a b c d : Expr)
     ]
   exact Expr.of_cancel_eq ctx a b c d
 
+/-- warning: declaration uses 'sorry' -/
+#guard_msgs in
+theorem Nat.Linear.Expr.of_cancel_eq_opt_denote' (ctx : Data.RArray Nat) (a b c d : Expr)
+  (h : Poly.cancel.rsimp (Expr.toNormPoly.rsimp a) (Expr.toNormPoly.rsimp b) = (Expr.toPolyFast.rsimp c, Expr.toPolyFast.rsimp d)) :
+  (Nat.Linear.Expr.denote' ctx a = Nat.Linear.Expr.denote' ctx b) =
+  (Nat.Linear.Expr.denote' ctx c = Nat.Linear.Expr.denote' ctx d) := by
+  sorry
+  all_goals
+  revert h
+  simp only [← Expr.toNormPoly.eq_rsimp, ← Expr.toPolyFast.eq_rsimp,
+    ← Poly.cancel.eq_rsimp, ← Nat.Linear.Expr.toPoly_eq_toPolyFast,
+    ← Nat.Linear.Expr.denote.eq_rsimp
+    ]
+  exact Expr.of_cancel_eq ctx a b c d
+
+/-- warning: declaration uses 'sorry' -/
+#guard_msgs in
+theorem Nat.Linear.Expr.of_cancel_eq_opt_denote'_no_rfl (ctx : Data.RArray Nat) (a b c d : Expr)
+  (h : True) :
+  (Nat.Linear.Expr.denote' ctx a = Nat.Linear.Expr.denote' ctx b) =
+  (Nat.Linear.Expr.denote' ctx c = Nat.Linear.Expr.denote' ctx d) := by
+  sorry
+
 open Lean Meta
 
 def bench (variant : Nat) : MetaM Unit :=
   let n := 40
   let decls := Array.ofFn fun (i : Fin n) => ((`x).appendIndexAfter i, (fun _ => pure (mkConst ``Nat)))
   withLocalDeclsD decls fun xs => do
-    let mut e₁ := Expr.num 42
-    let mut e₂ := Expr.num 23
-    for _ in [:4] do
-      for i in [:xs.size] do
-        e₁ := .add (.mulL i e₁) (.var i)
-        e₂ := .add (.var i) (Expr.mulR e₂ (xs.size - i))
+    if h : 0 < xs.size then
+      let mut e₁ := Expr.num 42
+      let mut e₂ := Expr.num 23
+      for _ in [:4] do
+        for i in [:xs.size] do
+          e₁ := .add (.mulL i e₁) (.var i)
+          e₂ := .add (.var i) (Expr.mulR e₂ (xs.size - i))
 
-    let (p₁', p₂') := Poly.cancel e₁.toNormPoly e₂.toNormPoly
-    let e₁' := p₁'.toExpr
-    let e₂' := p₂'.toExpr
-    have _value_orig := mkApp6 (.const ``Expr.of_cancel_eq [])
-      (← mkListLit (mkConst ``Nat) xs.toList)
-      (toExpr e₁) (toExpr e₂) (toExpr e₁') (toExpr e₂')
-      (← mkEqRefl (toExpr (p₁', p₂')))
-    have _value_no_rfl := mkApp5 (.const ``Expr.of_cancel_eq_no_rfl [])
-      (← mkListLit (mkConst ``Nat) xs.toList)
-      (toExpr e₁) (toExpr e₂) (toExpr e₁') (toExpr e₂')
-    have _value_opt := mkApp6 (.const ``Expr.of_cancel_eq_opt [])
-      (← mkListLit (mkConst ``Nat) xs.toList)
-      (toExpr e₁) (toExpr e₂) (toExpr e₁') (toExpr e₂')
-      (← mkEqRefl (toExpr (p₁', p₂')))
-    have _value_opt_denote := mkApp6 (.const ``Expr.of_cancel_eq_opt_denote [])
-      (← mkListLit (mkConst ``Nat) xs.toList)
-      (toExpr e₁) (toExpr e₂) (toExpr e₁') (toExpr e₂')
-      (← mkEqRefl (toExpr (p₁', p₂')))
-    let value := match variant with
-      | 0 => _value_orig
-      | 1 => _value_no_rfl
-      | 2 => _value_opt
-      | _ => _value_opt_denote
-    let value ← mkLambdaFVars xs value
-    let exp₁ ← Linear.Nat.LinearExpr.toArith xs e₁
-    let exp₂ ← Linear.Nat.LinearExpr.toArith xs e₂
-    let exp₁' ← Linear.Nat.LinearExpr.toArith xs e₁'
-    let exp₂' ← Linear.Nat.LinearExpr.toArith xs e₂'
-    let type ← mkEq (← mkEq exp₁ exp₂) (← mkEq exp₁' exp₂')
-    let type ← mkForallFVars xs type
+      let (p₁', p₂') := Poly.cancel e₁.toNormPoly e₂.toNormPoly
+      let e₁' := p₁'.toExpr
+      let e₂' := p₂'.toExpr
+      have _value_orig := mkApp6 (.const ``Expr.of_cancel_eq [])
+        (← mkListLit (mkConst ``Nat) xs.toList)
+        (toExpr e₁) (toExpr e₂) (toExpr e₁') (toExpr e₂')
+        (← mkEqRefl (toExpr (p₁', p₂')))
+      have _value_no_rfl := mkApp5 (.const ``Expr.of_cancel_eq_no_rfl [])
+        (← mkListLit (mkConst ``Nat) xs.toList)
+        (toExpr e₁) (toExpr e₂) (toExpr e₁') (toExpr e₂')
+      have _value_opt := mkApp6 (.const ``Expr.of_cancel_eq_opt [])
+        (← mkListLit (mkConst ``Nat) xs.toList)
+        (toExpr e₁) (toExpr e₂) (toExpr e₁') (toExpr e₂')
+        (← mkEqRefl (toExpr (p₁', p₂')))
+      have _value_opt_denote := mkApp6 (.const ``Expr.of_cancel_eq_opt_denote [])
+        (← mkListLit (mkConst ``Nat) xs.toList)
+        (toExpr e₁) (toExpr e₂) (toExpr e₁') (toExpr e₂')
+        (← mkEqRefl (toExpr (p₁', p₂')))
+      have _value_opt_denote' := mkApp6 (.const ``Expr.of_cancel_eq_opt_denote' [])
+        (Data.RArray.toExpr (mkConst ``Nat) id (.ofArray xs h))
+        (toExpr e₁) (toExpr e₂) (toExpr e₁') (toExpr e₂')
+        (← mkEqRefl (toExpr (p₁', p₂')))
+      have _value_opt_denote'_no_rfl := mkApp6 (.const ``Expr.of_cancel_eq_opt_denote'_no_rfl [])
+        (Data.RArray.toExpr (mkConst ``Nat) id (.ofArray xs h))
+        (toExpr e₁) (toExpr e₂) (toExpr e₁') (toExpr e₂')
+        (mkConst ``True.intro)
+      let value := match variant with
+        | 0 => _value_orig
+        | 1 => _value_no_rfl
+        | 2 => _value_opt
+        | 3 => _value_opt_denote
+        | 4 => _value_opt_denote'
+        | _ => _value_opt_denote'_no_rfl
+      let value ← mkLambdaFVars xs value
+      let exp₁ ← Linear.Nat.LinearExpr.toArith xs e₁
+      let exp₂ ← Linear.Nat.LinearExpr.toArith xs e₂
+      let exp₁' ← Linear.Nat.LinearExpr.toArith xs e₁'
+      let exp₂' ← Linear.Nat.LinearExpr.toArith xs e₂'
+      let type ← mkEq (← mkEq exp₁ exp₂) (← mkEq exp₁' exp₂')
+      let type ← mkForallFVars xs type
 
-    let name := `linear_test
-    let timings : List Nat ← (List.range 5).mapM fun _ =>
-      withoutModifyingEnv do
+      let name := `linear_test
       let decl := .thmDecl { name, value, type, levelParams := [] }
-      let start ← IO.monoMsNow
-      addDecl decl
-      return (← IO.monoMsNow) - start
-    let some best := timings.min? | unreachable!
-    logInfo m!"time {variant}: {best}ms"
-    -- logInfo m!"{type}"
+      let timings : List Nat ← (List.range 5).mapM fun _ =>
+        withoutModifyingEnv do
+          let start ← IO.monoMsNow
+          addDecl decl
+          return (← IO.monoMsNow) - start
+      let some best := timings.min? | unreachable!
+      logInfo m!"time {variant}: {best}ms"
+      -- logInfo m!"{type}"
+    else
+      unreachable!
 
-run_meta bench 0
-run_meta bench 1
+-- run_meta bench 0
+-- run_meta bench 1
 run_meta bench 2
 run_meta bench 3
+run_meta bench 4
+run_meta bench 5
